src/MutableMap/MutableMapFeasability.dfy
@@ -1,5 +1,3 @@
-include "MutableMap.dfy"
-
 /*******************************************************************************
 *  Copyright by the contributors to the Dafny Project
 *  SPDX-License-Identifier: MIT
@@ -7,46 +5,10 @@ include "MutableMap.dfy"
 
 // RUN: %dafny /compile:0 "%s"
 
-module {:options "/functionSyntax:4"} MutableMapTrait {
-  trait MutableMapTrait<K(==),V(==)> {
-    function content(): map<K, V>
-      reads this
-
-    method Put(k: K, v: V)
-      modifies this
-      ensures this.content() == old(this.content())[k := v]    
-
-    function Keys(): (keys: set<K>)
-      reads this
-      ensures keys == this.content().Keys
-
-    function Values(): (values: set<V>)
-      reads this
-      ensures values == this.content().Values
-
-    function Items(): (items: set<(K,V)>)
-      reads this
-      ensures items == this.content().Items
-      ensures items == set k | k in this.content().Keys :: (k, this.content()[k])
-
-    function Find(k: K): (v: V)
-      reads this
-      requires k in this.Keys()
-      ensures v in this.content().Values
-      ensures this.content()[k] == v
-    
-    method Remove(k: K)
-      modifies this
-      ensures this.content() == old(this.content()) - {k}
-
-    function Size(): (size: int)
-      reads this
-      ensures size == |this.content().Items|
-  }
-}
-
-module {:options "/functionSyntax:4"} MutableMapFeasability refines MutableMapTrait {
-  class MutableMap<K(==),V(==)> extends MutableMapTrait<K,V> {
+include "MutableMap.dfy"
+   
+module {:options "-functionSyntax:4"} MutableMapDafny refines MutableMap {
+  class MutableMapDafny<K(==),V(==)> extends MutableMap<K,V> {
     var m: map<K,V>
 
     function content(): map<K, V> 
@@ -56,6 +18,7 @@ module {:options "/functionSyntax:4"} MutableMapFeasability refines MutableMapTr
     }
 
     constructor ()
+      ensures this.content() == map[]
     {
       m := map[];
     }
@@ -72,6 +35,13 @@ module {:options "/functionSyntax:4"} MutableMapFeasability refines MutableMapTr
       ensures keys == this.content().Keys
     {
       m.Keys
+    }
+
+    predicate HasKey(k: K)
+      reads this
+      ensures HasKey(k) <==> k in this.content().Keys
+    {
+      k in m.Keys
     }
 
     function Values(): (values: set<V>)
@@ -100,9 +70,9 @@ module {:options "/functionSyntax:4"} MutableMapFeasability refines MutableMapTr
       items
     }
 
-    function Find(k: K): (v: V)
+    function Select(k: K): (v: V)
       reads this
-      requires k in this.Keys()
+      requires this.HasKey(k)
       ensures v in this.content().Values
       ensures this.content()[k] == v
     {
